Analysis.v
@@ -33,7 +33,14 @@ Inductive anni (A:Type) : Type :=
 | anni0 : anni A
 | anni1 (a1:A) : anni A
 | anni2 (a1:A) (a2:A) : anni A
+| anniF (a1:list A) (a2:A) : anni A
 | anni2opt (a1:option A) (a2:option A) : anni A.
+
+Definition anni_getF A (a:anni A) : list A :=
+  match a with
+    | anniF a1 s2 => a1
+    | _ => nil
+  end.
 
 Arguments anni A.
 Arguments anni0 [A].
@@ -43,6 +50,7 @@ Fixpoint setAnni {A} (a:ann A) (ai:anni A) : ann A :=
   match a, ai with
     | ann1 a an, anni1 a1 => ann1 a (setTopAnn an a1)
     | ann2 a an1 an2, anni2 a1 a2 => ann2 a (setTopAnn an1 a1) (setTopAnn an2 a2)
+    | annF a an1 an2, anniF a1 a2 => annF a (zip (@setTopAnn _) an1 a1) (setTopAnn an2 a2)
     | an, _ => an
   end.
 
@@ -50,16 +58,16 @@ Definition backward Dom FunDom
            (btransform : list FunDom -> stmt -> anni Dom -> Dom)
            (bmkFunDom : params -> ann Dom -> FunDom) :=
   fix backward
-         (st:stmt) (AL:list FunDom) (a:ann Dom) {struct st} : ann Dom :=
+         (AL:list FunDom) (st:stmt) (a:ann Dom) {struct st} : ann Dom :=
   match st, a with
     | stmtLet x e s as st, ann1 d ans =>
-      let ans' := backward s AL ans in
+      let ans' := backward AL s ans in
       let ai := anni1 (getAnn ans') in
       let d := (btransform AL st ai) in
       ann1 d ans'
     | stmtIf x s t as st, ann2 d ans ant =>
-      let ans' := backward s AL ans in
-      let ant' := backward t AL ant in
+      let ans' := backward AL s ans in
+      let ant' := backward AL t ant in
       let ai := anni2 (getAnn ans') (getAnn ant') in
       let d' := (btransform AL st ai) in
       ann2 d' ans' ant'
@@ -71,48 +79,54 @@ Definition backward Dom FunDom
       ann0 (btransform AL st anni0)
 
     | stmtExtern x f Y s as st, ann1 d ans =>
-      let ans' := backward s AL ans in
+      let ans' := backward AL s ans in
       let ai := anni1 (getAnn ans') in
       let d' := (btransform AL st ai) in
       ann1 d' ans'
-    | stmtFun Z s t as st, ann2 d ans ant =>
-      let ans' := backward s (bmkFunDom Z ans::AL) ans in
-      let ant' := backward t (bmkFunDom Z ans'::AL) ant in
-      let ai := anni2 (getAnn ans') (getAnn ant') in
-      let d' := btransform (bmkFunDom Z ans'::AL) st ai in
-      ann2 d' ans' ant'
+    | stmtFun F t as st, annF d ans ant =>
+      let ans' := zip (fun Zs =>
+        backward (zip (fun Zs ans => bmkFunDom (fst Zs) ans) F ans ++ AL) (snd Zs)) F ans in
+      let AL' := zip (fun Zs ans => bmkFunDom (fst Zs) ans) F ans' ++ AL in
+      let ant' := backward AL' t ant in
+      let ai := anniF (List.map getAnn ans') (getAnn ant') in
+      let d' := btransform AL' st ai in
+      annF d' ans' ant'
     | _, an => an
   end.
 
-
+(*
 Definition forward Dom FunDom
-         (ftransform : stmt -> (list FunDom * Dom) -> (list FunDom * anni Dom))
+         (ftransform : (list FunDom * Dom) -> stmt -> (list FunDom * anni Dom))
          (fmkFunDom : params -> ann Dom -> FunDom) :=
   fix forward
       (st:stmt) (a:list FunDom * ann Dom) {struct st}
 : list FunDom * ann Dom :=
   match st, a with
     | stmtLet x e s as st, (AL, ann1 d ans) =>
-      let (AL', ai) := (ftransform st (AL, d)) in
+      let (AL', ai) := (ftransform (AL, d) st) in
       forward s (AL', setAnni ans ai)
     | stmtIf x s t as st, (AL, ann2 d ans ant) =>
-      let (AL, ai) := (ftransform st (AL, d)) in
+      let (AL, ai) := (ftransform (AL, d) st) in
       let (AL', ans') := forward s (AL, setAnni ans ai) in
       let (AL'', ant') := forward t (AL', setAnni ant ai) in
       (AL'', ann2 d ans' ant')
     | stmtApp f Y as st, (AL, ann0 d as an) =>
-      let (AL', ai) := ftransform st (AL, d) in
+      let (AL', ai) := ftransform (AL, d) st in
       (AL', an)
     | stmtReturn x as st, (AL, ann0 d as an) =>
-      let (AL', ai) := ftransform st (AL, d) in
+      let (AL', ai) := ftransform (AL, d) st in
       (AL', an)
     | stmtExtern x f Y s as st, (AL, ann1 d ans) =>
-      let (AL, ai) := (ftransform st (AL, d)) in
+      let (AL, ai) := (ftransform (AL, d) st) in
       forward s (AL, setAnni ans ai)
-    | stmtFun Z s t as st, (AL, ann2 d ans ant) =>
-      let (AL, ai) := ftransform st (fmkFunDom Z ans::AL, d) in
-      let (AL', ans') := forward s (fmkFunDom Z (setAnni ans ai)::AL, setAnni ans ai) in
-      let (AL'', ant') := forward t (fmkFunDom Z ans'::AL', setAnni ant ai) in
+    | stmtFun F t as st, (AL, annF d ans ant) =>
+      let (AL, ai) := ftransform ((zip (fun Zs ans => fmkFunDom (fst Zs) ans) F ans++AL), d) st in
+      let AL1 := zip (fun Zs ans =>
+        fmkFunDom (fst Zs) ans) F (zip (@setTopAnn _) ans (anni_getF ai)) ++ AL in
+      let (AL', ans') := forward st (AL1, zip (@setTopAnn _) ans (anni_getF ai)) in
+      let AL2 := zip (fun Zs ans =>
+        fmkFunDom (fst Zs) ans) F ans' ++ AL' in
+      let (AL'', ant') := forward (AL2, setAnni ant ai) in
       (tl AL'', ann2 d ans' ant')
     | _, an => an
   end.
@@ -122,16 +136,17 @@ Definition makeForwardAnalysis Dom FunDom (BSL:BoundedSemiLattice Dom)
          (fmkFunDom : params -> ann Dom -> FunDom)
 : Analysis (ann Dom) :=
 makeAnalysis _ (fun s d => Success (snd (forward ftransform fmkFunDom s (nil, d)))) (fun s => setAnn s bottom).
+*)
 
 Definition makeBackwardAnalysis Dom FunDom (BSL:BoundedSemiLattice Dom)
            (btransform : list FunDom -> stmt -> anni Dom -> Dom)
            (bmkFunDom : params -> ann Dom -> FunDom)
 : Analysis (ann Dom) :=
 makeAnalysis _
-             (fun s d => Success (backward btransform bmkFunDom s nil d))
-             (fun s => setAnn s bottom).
+             (fun s d => Success (backward btransform bmkFunDom nil s d))
+             (fun s => setAnn bottom s).
 Module SSA.
-
+(*
 Definition forward Dom {BSL:BoundedSemiLattice Dom} FunDom
          (ftransform : stmt -> (list FunDom * Dom) -> (list FunDom * anni Dom))
          (fmkFunDom : params -> Dom -> FunDom)
@@ -182,6 +197,7 @@ Definition forward Dom {BSL:BoundedSemiLattice Dom} FunDom
         | _ => Error "function binding transformer failed"
       end
   end.
+ *)
 
 (*
 Lemma forward_FunDom_length Dom {BSL:BoundedSemiLattice Dom} FunDom
@@ -218,14 +234,14 @@ Definition forward Dom FunDom
       forward t (forward s( ftransform st (fmkFunDom Z d::AL, d)))
   end.
 *)
-
+(*
 Definition makeForwardAnalysis Dom FunDom (BSL:BoundedSemiLattice Dom) (PO:PartialOrder FunDom)
          (ftransform : stmt -> (list FunDom * Dom) -> (list FunDom * anni Dom))
          (fmkFunDom : params -> Dom -> FunDom)
          fgetDom
 : Analysis (list FunDom * Dom) :=
 makeAnalysis _ (fun s d => forward ftransform fmkFunDom fgetDom s d) (fun s => (nil, bottom)).
-
+*)
 
 (*
 Definition makeBackwardAnalysis Dom FunDom (BSL:BoundedSemiLattice Dom)
